theories/eris/lib/sampling/geometric/interface.v
@@ -1,100 +1,164 @@
 From clutch.eris Require Export eris.
-From clutch.eris.lib.sampling Require Import utils. 
+From clutch.eris.lib.sampling Require Import distr_impl utils. 
 
-Definition geometric_prob (p q k : nat) :=  (p / (q + 1) * (1 - p / (q + 1))^k)%R.
+Section GeometricMath.
 
-Lemma geometric_prob_pos (p q k : nat) : p ≤ S q → (0 <= geometric_prob p q k)%R.
-Proof.
-  move=>p_le_Sq.
-  apply le_INR in p_le_Sq.
-  rewrite S_INR in p_le_Sq.
-  unfold geometric_prob.
-  pose proof (pos_INR p).
-  pose proof (pos_INR q).
-  apply Rmult_le_pos.
-  { apply Rcomplements.Rdiv_le_0_compat; lra. }
-  { apply pow_le.
-    apply Rle_0_le_minus.
-    rewrite -Rcomplements.Rdiv_le_1; lra.
-  }
-Qed.
+  Definition geometric_prob (p q k : nat) :=  (p / (q + 1) * (1 - p / (q + 1))^k)%R.
+  
+  Lemma geometric_prob_pos (p q k : nat) : p ≤ S q → (0 <= geometric_prob p q k)%R.
+  Proof.
+    move=>p_le_Sq.
+    apply le_INR in p_le_Sq.
+    rewrite S_INR in p_le_Sq.
+    unfold geometric_prob.
+    pose proof (pos_INR p).
+    pose proof (pos_INR q).
+    apply Rmult_le_pos.
+    { apply Rcomplements.Rdiv_le_0_compat; lra. }
+    { apply pow_le.
+      apply Rle_0_le_minus.
+      rewrite -Rcomplements.Rdiv_le_1; lra.
+    }
+  Qed.
 
-Lemma geometric_prob_S (p q k : nat) : (geometric_prob p q (S k) = (1 - p / (q + 1)) * geometric_prob p q k)%R.
-Proof.
-  unfold geometric_prob.
-  simpl.
-  lra.
-Qed.
+  Lemma geometric_prob_S (p q k : nat) : (geometric_prob p q (S k) = (1 - p / (q + 1)) * geometric_prob p q k)%R.
+  Proof.
+    unfold geometric_prob.
+    simpl.
+    lra.
+  Qed.
 
-Lemma is_seriesC_geometric_prob (p q : nat) : 0 < p ≤ S q → is_seriesC (geometric_prob p q) 1%R.
-Proof.
-  move=>[p_pos p_le_Sq].
-  apply le_INR in p_le_Sq.
-  rewrite S_INR in p_le_Sq.
-  apply lt_INR in p_pos.
-  simpl in p_pos.
-  unfold geometric_prob.
-  replace 1%R with (p / (q + 1) * ((q + 1) / p))%R at 1; last first.
-  { rewrite !Rdiv_def Rmult_comm -Rmult_assoc (Rmult_assoc _ _ p) Rinv_l; last lra.
-    rewrite Rmult_1_r Rinv_r; lra.
-  }
-  apply is_seriesC_scal_l.
-  apply is_seriesC_is_series_nat.
-  replace ((q + 1) / p)%R with (/ (1 - (1 - p / (q + 1))))%R; last first.
-  { rewrite Rminus_def Ropp_plus_distr Ropp_involutive
-            -Rplus_assoc -Rminus_def Rminus_diag Rplus_0_l Rinv_div //.
-  }
-  apply Series.is_series_geom.
-  apply Rabs_def1.
-  { apply Rcomplements.Rlt_minus_l.
-    rewrite -{1}(Rplus_0_r 1).
-    apply Rplus_le_lt_compat; first reflexivity.
-    apply Rcomplements.Rdiv_lt_0_compat; lra.
-  }
-  { apply (Rlt_le_trans _ 0%R); first lra.
-    apply Rle_0_le_minus.
-    rewrite -Rcomplements.Rdiv_le_1; lra.
-  }
-Qed.
+  Lemma is_seriesC_geometric_prob (p q : nat) : 0 < p ≤ S q → is_seriesC (geometric_prob p q) 1%R.
+  Proof.
+    move=>[p_pos p_le_Sq].
+    apply le_INR in p_le_Sq.
+    rewrite S_INR in p_le_Sq.
+    apply lt_INR in p_pos.
+    simpl in p_pos.
+    unfold geometric_prob.
+    replace 1%R with (p / (q + 1) * ((q + 1) / p))%R at 1; last first.
+    { rewrite !Rdiv_def Rmult_comm -Rmult_assoc (Rmult_assoc _ _ p) Rinv_l; last lra.
+      rewrite Rmult_1_r Rinv_r; lra.
+    }
+    apply is_seriesC_scal_l.
+    apply is_seriesC_is_series_nat.
+    replace ((q + 1) / p)%R with (/ (1 - (1 - p / (q + 1))))%R; last first.
+    { rewrite Rminus_def Ropp_plus_distr Ropp_involutive
+              -Rplus_assoc -Rminus_def Rminus_diag Rplus_0_l Rinv_div //.
+    }
+    apply Series.is_series_geom.
+    apply Rabs_def1.
+    { apply Rcomplements.Rlt_minus_l.
+      rewrite -{1}(Rplus_0_r 1).
+      apply Rplus_le_lt_compat; first reflexivity.
+      apply Rcomplements.Rdiv_lt_0_compat; lra.
+    }
+    { apply (Rlt_le_trans _ 0%R); first lra.
+      apply Rle_0_le_minus.
+      rewrite -Rcomplements.Rdiv_le_1; lra.
+    }
+  Qed.
 
+  Program Definition geometric_distr (p q : nat) (p_bounds : 0 < p ≤ S q) : distr nat
+    := MkDistr
+         (geometric_prob p q)
+         (λ k, geometric_prob_pos p q k (proj2 p_bounds))
+         (ex_intro _ _ (is_seriesC_geometric_prob p q p_bounds))
+         _ .
+  Next Obligation.
+    move=>p q p_bounds.
+    rewrite (is_seriesC_unique _ _ (is_seriesC_geometric_prob p q p_bounds)) //.
+  Qed.
+
+End GeometricMath.
 
 Class geometric_spec (geometric_prog geometric_alloc : val) :=
   GeometricSpec
-  {
-    twp_geometric_adv_comp  `{!erisGS Σ} :
-    ∀ (p q : nat),
-      (0 < p)%nat →
-      (p ≤ q + 1)%nat →
-      ∀ (D : nat → R) (L : R) (ε : R),
-      (∀ (n : nat), 0 <= D n <= L)%R →
-      SeriesC (λ k, (geometric_prob p q k * D k)%R) = ε →
-      ↯ ε -∗ WP geometric_prog #() #p #q [{ v, ∃ (k : nat), ⌜v = #k⌝ ∗ ↯ (D k) }];
+    {
+      twp_geometric_adv_comp `{!erisGS Σ} :
+      ∀ (p q : nat),
+        (0 < p)%nat →
+        (p ≤ q + 1)%nat →
+        ∀ (D : nat → R) (L : R) (ε : R),
+        (∀ (n : nat), 0 <= D n <= L)%R →
+        SeriesC (λ k, (geometric_prob p q k * D k)%R) = ε →
+        ↯ ε -∗ WP geometric_prog #() #p #q [{ v, ∃ (k : nat), ⌜v = #k⌝ ∗ ↯ (D k) }];
 
-    own_geometric_tape `{!erisGS Σ} (α : loc) (N M : nat) (v : list nat) : iProp Σ;
+      own_geometric_tape `{!erisGS Σ} (α : loc) (N M : nat) (v : list nat) : iProp Σ;
 
-    twp_geometric_alloc `{!erisGS Σ} (p q : nat) :
+      twp_geometric_alloc `{!erisGS Σ} (p q : nat) :
       [[{ True }]]
         geometric_alloc #p #q
-      [[{ (α : loc), RET #lbl:α; own_geometric_tape α p q [] }]];
-    
-    twp_geometric_tape `{!erisGS Σ} :
-    ∀ (p q r : nat) (α : loc) (n : nat) (ns : list nat) (Φ : val → iProp Σ),
-      own_geometric_tape α p q (n::ns) -∗
-      (own_geometric_tape α p q ns -∗ Φ #n) -∗
-      WP geometric_prog #lbl:α #p #q #r [{ Φ }];
- 
-    twp_geometric_presample_adv_comp `{!erisGS Σ} :
-    ∀ (p q : nat) (α : loc) (l : list nat) (e : expr) (Φ : val → iProp Σ),
-      0 < p →
-      p ≤ (q + 1) →
-      to_val e = None →
-      ∀ (r : nat) (D : nat → R) (L : R) (ε : R),
-      (∀ (n : nat), 0 <= D n <= L)%R →
-      SeriesC (λ k, (geometric_prob p q k * D k)%R) = ε →
-      ↯ ε ∗
-      own_geometric_tape α p q l ∗
-      (∀ (n : nat),
-         ↯ (D n) -∗
-         own_geometric_tape α p q (l ++ [n]) -∗ WP e [{ Φ }]) ⊢
-      WP e [{ Φ }]
-  }.
+        [[{ (α : loc), RET #lbl:α; own_geometric_tape α p q [] }]];
+      
+      twp_geometric_tape `{!erisGS Σ} :
+      ∀ (p q : nat) (α : loc) (n : nat) (ns : list nat) (Φ : val → iProp Σ),
+        own_geometric_tape α p q (n::ns) -∗
+        (own_geometric_tape α p q ns -∗ Φ #n) -∗
+        WP geometric_prog #lbl:α #p #q [{ Φ }];
+      
+      twp_geometric_presample_adv_comp `{!erisGS Σ} :
+      ∀ (p q : nat) (α : loc) (ns : list nat)
+        (e : expr) 
+        (D : nat → R) (L : R) (ε : R)
+        (Φ : val → iProp Σ),
+        (0 < p)%nat →
+        (p ≤ q + 1)%nat →
+        to_val e = None → 
+        (∀ (n : nat), 0 <= D n <= L)%R →
+        SeriesC (λ k, (geometric_prob p q k * D k)%R) = ε →
+        own_geometric_tape α p q ns ∗
+        ↯ ε ∗ 
+        (∀ (i : nat), ↯ (D i) ∗ own_geometric_tape α p q (ns ++ [i]) -∗ WP e [{ Φ }])
+        ⊢  WP e [{ Φ }]
+    }.
+
+Section GeometricInst.
+
+  Context `{geospec : geometric_spec geo geoalloc}.
+  
+  Instance geometric_binomial_impl {p q : nat} {p_bounds : 0 < p ≤ S q} :
+    distr_impl (dmap (LitV ∘ LitInt ∘ Z.of_nat) (geometric_distr p q p_bounds)).
+  Proof using geospec.
+
+    refine (MkDistrImpl _
+              (λ: "α", geo "α" #p #q) (geoalloc #p #q)
+              loc
+              (λ _ _ Δ l, ∃ l', own_geometric_tape Δ p q l' ∗
+                            ⌜l = fmap (λ (k : nat), #k) l'⌝)%I
+              (λ _ _ Δ α, ⌜α = #lbl:Δ⌝)%I #() _ _ _ _).
+    - iIntros (Σ erisGS0 D ε L ε_ge_0 D_bounds D_sum Φ) "Herr HΦ".
+      set (D' (k : nat) := D #k).
+      wp_pures.
+      iPoseProof (twp_geometric_adv_comp p q (proj1 p_bounds) ltac:(lia) D' L _ _ with "Herr") as "HH".
+      Unshelve.
+      3:{ move=>k. apply D_bounds. }
+      { rewrite (dmap_expected_value _ _ _ L) // in D_sum. }
+      wp_apply tgl_wp_wand_r.
+      iFrame.
+      iIntros (?) "(%k & -> & Herr)".
+      by iApply "HΦ".
+    - iIntros (Σ erisGS0 Φ) "_ HΦ".
+      wp_apply (twp_geometric_alloc with "[$]") as (α) "Hα".
+      iApply "HΦ".
+      by iFrame.
+    - iIntros (Σ erisGS0 e ε Δ l D L Φ e_not_val ε_ge_0 D_bounds D_sum) "(Herr & (%l' & Htape & ->) & Hnext)".
+      set (D' (k : nat) := D #k).
+      wp_apply (twp_geometric_presample_adv_comp p q _ _ _ D' _ _ _ (proj1 p_bounds) ltac:(lia) e_not_val with "[$Herr $Htape Hnext]").
+      { move=>k. apply D_bounds. }
+      { rewrite (dmap_expected_value _ _ _ L) // in D_sum. }
+      iIntros (k) "[Herr Htape]".
+      wp_apply "Hnext".
+      iFrame.
+      rewrite fmap_app //.
+    - iIntros (Σ erisGS0 α Δ l v Φ) "[(%l' & Htape & %Heq) ->] HΦ".
+      destruct l' as [|v' l']; first discriminate.
+      injection Heq as -> ->.
+      wp_pures.
+      wp_apply (twp_geometric_tape with "Htape") as "Htape".
+      iApply "HΦ".
+      iExists l'.
+      by iFrame.
+  Defined.
+
+End GeometricInst.
